Domain.lean
@@ -14,5 +14,6 @@ import Domain.Neighborhood.Example12
 import Domain.Neighborhood.Example13
 import Domain.Neighborhood.Example14
 import Domain.Neighborhood.Example15
+import Domain.Neighborhood.ExampleB
 import Domain.Neighborhood.Exercise122
 import Domain.InfoSys
